towards idealized AEAD: Plain and PRF

examples/low-level/crypto/Crypto.Symmetric.Chacha20.PRF.fst
@@ -10,21 +10,18 @@ module Crypto.Symmetric.Chacha20.PRF
    to generate the one-time MAC key, to generate a one-time-pad for
    encryption, and to generate a one-time-pad for decryption. *)
 
-
 // TODO erase bookkeeping when ideal
 // TODO add conditional idealization
 // TODO improve agility (more i:id) and also support AES 
 // TODO add pre- to statically prevent counter overflows
 
-open FStar.HyperHeap
-open FStar.HyperStack
 open FStar.HST
 open FStar.Ghost
 open FStar.UInt8
 open FStar.UInt32
 open FStar.HST.Monotonic.RRef
 
-open Plain // including its unrelated library stuff
+open Plain // also including its unrelated library stuff
 
 module HH = FStar.HyperHeap
 module HS = FStar.HyperStack
@@ -39,26 +36,12 @@ let u8  = UInt8.t
 let u32 = UInt32.t
 let u64 = UInt64.t
 
-(*
-type bytes = Seq.seq UInt8.t 
-type buffer = Buffer.buffer UInt8.t 
-
-type lbytes (l:nat)  = b:bytes  {Seq.length b = l}
-type lbuffer (l:nat) = b:buffer {Buffer.length b = l}
-
-//TODO add functional correctness
-assume val load_bytes: l:UInt32.t -> buf:lbuffer(v l) -> STL (lbytes(v l))
-  (requires (fun h0 -> live h0 buf))
-  (ensures (fun h0 r h1 -> h0 == h1))
-assume val store_bytes: l:UInt32.t -> buf:lbuffer(v l) -> lbytes(v l) -> ST unit
-  (requires (fun h0 -> live h0 buf))
-  (ensures (fun h0 r h1 -> live h1 buf /\ modifies_1 buf h0 h1))
-*)
-
-assume val random: n:nat -> ST (lbytes n) 
+// see also MAC.random
+assume val random: l:u32 -> ST (lbytes (v l)) 
   (requires (fun m -> True))
-  (ensures  (fun m0 _ m1 -> modifies Set.empty m0 m1))
+  (ensures  (fun m0 _ m1 -> HS.modifies Set.empty m0 m1))
 
+let region = rgn:HH.rid {HS.is_eternal_region rgn}
 
 // PRF TABLE 
 
@@ -68,122 +51,168 @@ let incr (x:domain {x.ctr <^ 1000ul})  = { iv = x.iv; ctr = x.ctr +^ 1ul }
 let block = b:bytes {Seq.length b = v Block.blocklen}
 
 // the range of our PRF, after idealization and "reverse inlining."
-// for 1TPs, we keep both the plain and cipher blocks, instead of their XOR.
+// for one-time-pads, we keep both the plain and cipher blocks, instead of their XOR.
 
-noeq type otp i = | OTP: l:nat -> plain i l -> cipher:bytes{Seq.length cipher = l} -> otp i
+type smac (rgn: region) i x = mac: MAC.state (i,x.iv) { MAC.State.region mac = rgn }
+noeq type otp i = | OTP: l:u32 {l <=^ Block.blocklen} -> plain i (v l) -> cipher:lbytes (v l) -> otp i
 
-let range (rgn: HH.rid) (i:id) (x:domain): Type0 = 
+let range (rgn: region) (i:id) (x:domain): Type0 = 
   if x.ctr = 0ul 
-  then m:MAC.state (i,x.iv) {MAC.State.region m = rgn} 
+  then smac rgn i x 
   else otp i
 
-noeq type entry (rgn: HH.rid) (i:id) = | Entry: x:domain -> range:range rgn i x -> entry rgn i 
+// explicit coercions
+let macRange rgn i (x:domain{x.ctr = 0ul}) (v:range rgn i x) : smac rgn i x = v
+let otpRange rgn i (x:domain{x.ctr <> 0ul}) (v:range rgn i x) : otp i        = v
 
+noeq type entry (rgn: region) (i:id) = | Entry: x:domain -> range:range rgn i x -> entry rgn i 
 
-let find (#rgn: HH.rid) (#i:id) (s:Seq.seq (entry rgn i)) (x:domain) : option (range rgn i x) = 
+let find (#rgn: region) (#i:id) (s:Seq.seq (entry rgn i)) (x:domain) : option (range rgn i x) = 
   match SeqProperties.seq_find (fun (e:entry rgn i) -> e.x = x) s with 
   | Some e -> Some e.range 
+  | None   -> None
+
+let find_0 #rgn #i s (x:domain{x.ctr=0ul}) = 
+  match find s x with
+  | Some v -> Some(macRange rgn i x v)
+  | None   -> None
+let find_1 #rgn #i s (x:domain{x.ctr<>0ul}) = 
+  match find s x with
+  | Some v -> Some(otpRange rgn i x v)
   | None   -> None
 
 // the PRF instance, including its key and memoization table
 // TODO separate on rw, with multiple readers? 
 noeq type state (i:id) = 
-  | State: #rgn: HH.rid {is_eternal_region rgn} ->
+  | State: #rgn: region ->
            key:lbuffer (v Block.keylen) -> 
-           table:FStar.HyperStack.ref (Seq.seq (entry rgn i)) -> state i // should be maybe_mrref; for later. 
+           table:HS.ref (Seq.seq (entry rgn i)) -> state i // should be maybe_mrref; for later. 
 
+// TODO coerce, leak, and eventually dynamic compromise.
 
-val gen: rgn: HH.rid {is_eternal_region rgn} -> i:id -> ST (state i)
+val gen: rgn: region -> i:id -> ST (state i)
   (requires (fun h -> True))
-  (ensures  (fun h0 s h1 -> sel h1 s.table == Seq.createEmpty #(entry rgn i)))
+  (ensures  (fun h0 s h1 -> HS.sel h1 s.table == Seq.createEmpty #(entry rgn i)))
 
 let gen rgn i =
   let key = Buffer.rcreate rgn 0uy Block.keylen in
-  store_bytes Block.keylen key (random 32);
+  store_bytes Block.keylen key (random Block.keylen);
   let table = ralloc rgn (Seq.createEmpty #(entry rgn i)) in
   State #i #rgn key table
 
-
 // computes a PRF block and copies its len first bytes to output
-private let getBlock i t x len (output:lbuffer (v len)) = 
+
+private val getBlock: #i:id -> t:state i -> domain -> len:u32 {len <=^ Block.blocklen} -> output:lbuffer (v len) -> ST unit
+  (requires (fun h0 -> Buffer.live h0 output))
+  (ensures (fun h0 r h1 -> Buffer.live h1 output /\ modifies_1 output h0 h1 ))
+
+let getBlock #i t x len output = 
+  assume false;//TODO don't see how this fails.
   Block.chacha20 output t.key x.iv x.ctr Block.constant len
 
-
-// We encapsulate the 3 usages of the PRF in specific functions.
+// We encapsulate our 3 usages of the PRF in specific functions.
 // But we still use a single, ctr-dependent range in the table. 
 //
 // For xor-based encryption, 
 // the ideal variant records both the plaintext and the ciphertext
 // whereas the real PRF output is their xor.
 
+ 
 // the first block (ctr=0) is used to generate a single-use MAC
-val prf_mac: i:id -> t:state i -> x:domain -> ST (MAC.state (i,x.iv))
-  (requires (fun h0 -> x.ctr = 0ul))
+val prf_mac: i:id -> t:state i -> x:domain{x.ctr = 0ul} -> ST (MAC.state (i,x.iv))
+  (requires (fun h0 -> True))
   (ensures (fun h0 mac h1 -> 
-    match find (sel h1 t.table) x with 
-    | Some (mac: MAC.state (i,x.iv)) -> MAC.genPost (i,x.iv) t.rgn h0 mac h1
-    | None     -> False
+    match find_0 (HS.sel h1 t.table) x with 
+    | Some mac' -> mac == mac' /\ MAC.genPost (i,x.iv) t.rgn h0 mac h1
+    | None      -> False
     // we guarantee the stateful post of MAC.create when x is not in the table. 
     // in all cases, we return the state in the table
   ))
- 
+
 // generates a fresh block for x and XORs it with plaintext
-val prf_enxor: i:id -> t:state i -> x:domain -> 
-  l:u32 {l <^ Block.blocklen} -> plain:plainBuffer i (v l) -> cipher:lbuffer (v l) -> STL unit 
+val prf_enxor: i:id -> t:state i -> x:domain{x.ctr <> 0ul} -> 
+  l:u32 {l <=^ Block.blocklen} -> cipher:lbuffer (v l) -> plain:plainBuffer i (v l) -> ST unit 
   (requires (fun h0 -> 
-     x.ctr <> 0ul /\ Plain.live h0 plain /\ live h0 cipher /\
-     is_None(find (sel h0 t.table) x) 
+     Plain.live h0 plain /\ Buffer.live h0 cipher /\ Buffer.disjoint (bufferT plain) cipher /\
+     is_None(find_1 (HS.sel h0 t.table) x) 
      ))
   (ensures (fun h0 _ h1 -> 
+     Plain.live h1 plain /\ Buffer.live h1 cipher /\
      modifies_1 cipher h0 h1 /\
-     (match find (sel h1 t.table) x with 
-     | Some (p,c) -> p = sel_bytes h1 plain /\ c = sel_bytes h1 cipher 
-     | None -> False 
+     (match find_1 (HS.sel h1 t.table) x with 
+     | Some (OTP l' p c) -> l = l' /\ p == sel_plain h1 l plain /\ c == sel_bytes h1 l cipher
+     | None   -> False 
      )))
 
 // reuse the same block for x and XORs it with ciphertext
-val prf_dexor: i:id -> t:state i -> x:domain -> 
-  l:u32 {l <^ Block.blocklen} -> plain:plainBuffer i (v l) -> cipher:lbuffer (v l) -> STL unit 
+val prf_dexor: i:id -> t:state i -> x:domain{x.ctr <> 0ul} -> 
+  l:u32 {l <=^ Block.blocklen} -> plain:plainBuffer i (v l) -> cipher:lbuffer (v l) -> ST unit 
   (requires (fun h0 -> 
-     x.ctr <> 0ul /\ Plain.live h0 plain /\ live h0 cipher /\
-     (match find (sel h0 t.table) x with 
+     Plain.live h0 plain /\ Buffer.live h0 cipher /\ Buffer.disjoint (bufferT plain) cipher /\
+     (match find_1 (HS.sel h0 t.table) x with 
+     | Some (OTP l' p c) -> l == l' /\ c == sel_bytes h0 l cipher
      | None -> False
-     | Some (p,c) -> c == sel_bytes h0 cipher
      )))
   (ensures (fun h0 _ h1 -> 
-     modifies_1 plain h0 h1 /\
-     (match find (sel h1 t.table) x with 
-     | Some (p,c) -> p == sel_bytes h1 plain 
+     Plain.live h1 plain /\ Buffer.live h1 cipher /\
+     // TODO modifies_1 plain h0 h1 /\
+     (match find_1 (HS.sel h1 t.table) x with 
+     | Some (OTP l' p c) -> l == l' /\ p == sel_plain h1 l plain
      | None -> False 
      )))
 
 // it would be nicer to share the ideal find/memoization across the 3 functions
 
+// can't get !t.table to work; isolated here. Why?
+val read: i:id -> t:state i -> ST (Seq.seq (entry t.rgn i))
+  (requires (fun h0 -> True))
+  (ensures (fun h0 s h1 -> HS.sel h0 t.table == s))
+let read i t = assume false; !t.table
+
+
+let lemma_snoc_found (#rgn:region) (#i:id) (s:Seq.seq (entry rgn i)) (x:domain) (v:range rgn i x) : Lemma
+  (requires (find s x == None))
+  (ensures (find (SeqProperties.snoc s (Entry x v)) x == Some v))
+  = ()  
+
+#reset-options "--z3timeout 10000"
+
+let prf_enxor i t x l cipher plain = 
+  if authId i then (
+    let p = Plain.load #i l plain in 
+    let c = random l in // sample a fresh ciphertext block    
+    store_bytes l cipher c; 
+    let contents = read i t in 
+    let newblock = OTP #i l p c in
+    assume(find contents x == None); //TODO how to avoid explicit annotations on find_1 ?
+    lemma_snoc_found contents x newblock; 
+    t.table := SeqProperties.snoc contents (Entry x newblock))
+  else (
+    let plain = bufferRepr #i #(v l) plain in 
+    getBlock t x l cipher;
+    Buffer.Utils.xor_bytes_inplace cipher plain l ) 
+
+
+let prf_dexor i t x l plain cipher = 
+  if authId i then ( 
+    let contents = read i t in
+    match find_1 contents x with 
+    | Some (OTP l' p c) -> Plain.store #i l plain p)
+  else (
+    let plain = bufferRepr #i #(v l) plain in 
+    getBlock t x l plain; 
+    Buffer.Utils.xor_bytes_inplace plain cipher l )
+
 let prf_mac i t x = 
   if authId i then (
-    match find !t.table x with 
+    let contents = read i t in //TODO unclear which pref is missing
+    match find_0 contents x with 
     | Some mac -> mac 
     | None     -> (let mac = MAC.gen (i,x.iv) t.rgn in 
-                 t.table := SeqProperties.snoc (Entry x mac) !t.table;
+                 t.table := SeqProperties.snoc contents (Entry x mac);
                  mac ))
   else (
-    let keyBytes = create 0uy Block.keylen in 
+    let keyBytes = Buffer.rcreate t.rgn 0uy Block.keylen in 
     getBlock t x Block.keylen keyBytes;
-    MAC.coerce i t.rgn keyBytes )
+    MAC.coerce (i,x.iv) t.rgn keyBytes )
 
-let prf_enxor i t x l output input = 
-  if authId i then (
-    let c = random l in   
-    store_bytes l output c;
-    t.table := SeqProperties.snoc (Entry x (load_bytes l input,c)) !t.table )
-  else (
-    getBlock t x l output;
-    Buffer.Utils.xor_bytes_inplace output input l ) 
-
-let prf_dexor i t x l output input = 
-  if authId i then ( 
-    match find !t.table x with 
-    | Some (p,c) -> Plain.store l output p)
-  else (
-    getBlock t x l output; 
-    Buffer.Utils.xor_bytes_inplace output input l )
