examples/low-level/crypto/Plain.fst
@@ -18,6 +18,8 @@ open Buffer.Utils
 
 // LIBRARY STUFF
 
+type mem = FStar.HyperStack.mem
+
 let modifies_1 = Buffer.modifies_1
 
 type bytes = Seq.seq UInt8.t 
@@ -33,7 +35,7 @@ assume val load_bytes: l:UInt32.t -> buf:lbuffer(v l) -> STL (lbytes(v l))
 assume val store_bytes: l:UInt32.t -> buf:lbuffer(v l) -> lbytes(v l) -> ST unit
   (requires (fun h0 -> Buffer.live h0 buf))
   (ensures (fun h0 r h1 -> Buffer.live h1 buf /\ modifies_1 buf h0 h1))
-assume val sel_bytes: h:FStar.HyperHeap.t -> l:UInt32.t -> buf:lbuffer(v l) -> Tot (lbytes (v l))
+assume val sel_bytes: h:mem -> l:UInt32.t -> buf:lbuffer(v l){Buffer.live h buf}  -> Tot (lbytes (v l))
 // how to state that buf is live here?
 
 // SECRETS, HIGH AND LOW
@@ -45,23 +47,44 @@ type plainLen = nat // we'll need a tigher bound
 
 abstract type plain (i:id) (l:plainLen) = lbytes l
 
+// to be restricted
 val repr: #i:id -> #l:plainLen -> p:plain i l -> Tot (lbytes (Seq.length p))
 let repr #i #l p = p
 
 val make: #i:id -> l:plainLen -> b:lbytes l -> Tot (plain i l)
 let make #i l b = b
 
-open FStar.Buffer 
-
 abstract type plainBuffer (i:id) (l:plainLen) = b:lbuffer l
 
 let live #i #l h (p:plainBuffer i l) = Buffer.live h p
 
-let create (i:id) (zero:UInt8.t) (l:UInt32.t): plainBuffer i (v l)  = create zero l 
+let create (i:id) (zero:UInt8.t) (l:UInt32.t): plainBuffer i (v l) = Buffer.create zero l 
 
+open FStar.Buffer // for .idx
 let sub #id #l (b:plainBuffer id l) (i:UInt32.t{v i + v b.idx < pow2 n}) (len:UInt32.t{v len <= length b /\ v i + v len <= length b}) : Tot (b':plainBuffer id (v len))
   = sub b i len
 // ...
 
-let load #i l (buf: plainBuffer i (v l)): plain i (v l) = load_bytes l buf
-let store #i l (buf: plainBuffer i (v l)) (b: plain i (v l)) : unit = store_bytes l buf b
+
+val bufferT: #i:id -> #l:plainLen -> b:plainBuffer i l -> GTot (lbuffer l)
+let bufferT #i #l b = b
+
+val bufferRepr: #i:id {~(authId i)} -> #l:plainLen -> b:plainBuffer i l -> Tot (b':lbuffer l{ b' == bufferT b})
+let bufferRepr #i #l b = b
+// not sure how to write modifies clauses including plain and plainBuffer
+
+val load: #i:id -> l:UInt32.t -> buf: plainBuffer i (v l) -> STL (plain i (v l)) 
+  (requires (fun h0 -> live h0 buf))
+  (ensures (fun h0 r h1 -> h0 == h1))
+let load #i l buf = load_bytes l buf
+
+val store: #i:id -> l:UInt32.t -> buf: plainBuffer i (v l) -> b:plain i (v l) -> STL unit
+  (requires (fun h0 -> live h0 buf))
+  (ensures (fun h0 r h1 -> live h1 buf /\ modifies_1 (bufferT #i #(v l) buf) h0 h1
+  ))
+let store #i l buf b = 
+  assume false; // TODO, not sure what's missing here
+  store_bytes l buf b
+
+val sel_plain: h:mem -> #i:id -> l:UInt32.t -> buf:plainBuffer i (v l){live h buf} -> Tot (plain i (v l)) 
+let sel_plain h #i l buf = sel_bytes h l buf
